src/coqutil/Map/OfListWord.v
@@ -6,40 +6,44 @@ Require Import coqutil.Map.Properties.
 Require Import coqutil.Tactics.autoforward.
 Require Import coqutil.Tactics.Tactics.
 Import Interface.map MapKeys.map OfFunc.map.
-Require Import coqutil.Word.Interface coqutil.Word.Properties.
+From Stdlib Require Import Zmod Zmod.Bits.
+Require Import coqutil.Word.Properties.
 
 Module map.
   Section __. Local Set Default Proof Using "All".
-    Context {width} {word : word width} {word_ok : word.ok word}.
-    Add Ring __wring: (@word.ring_theory width word word_ok).
+    Context {width : Z} (Hw : (0 < width)%Z).
+    Local Notation word := (bits width).
+    Add Ring __wring: (Zmod.ring_theory (2 ^ width))
+        (preprocess [autorewrite with rew_word_morphism],
+         morphism (word.ring_morph (width := width)),
+         constants [word_cst]).
     Context {value : Type} {map : map word value} {ok : map.ok map}.
 
     Definition of_list_word (xs : list value) : map :=
       map.of_func
-      (fun w => nth_error xs (Z.to_nat (word.unsigned w)))
-      (List.map (fun n => word.of_Z (Z.of_nat n)) (seq 0 (length xs))).
+      (fun w => nth_error xs (Z.to_nat (Zmod.unsigned w)))
+      (List.map (fun n => bits.of_Z width (Z.of_nat n)) (seq 0 (length xs))).
     Definition of_list_word_at (a : word) (xs : list value) : map :=
-      map_keys (word.add a) (of_list_word xs).
+      map_keys (Zmod.add a) (of_list_word xs).
     Lemma get_of_list_word xs i : get (of_list_word xs) i
-      = nth_error xs (Z.to_nat (word.unsigned i)).
+      = nth_error xs (Z.to_nat (Zmod.unsigned i)).
     Proof.
-      pose proof (word.eqb_spec (word_ok:=word_ok)).
       cbv [of_list_word].
       erewrite get_of_func_Some_supported; trivial; intros.
-      pose proof word.unsigned_range k.
-      eapply in_map_iff; exists (Z.to_nat (word.unsigned k));
+      pose proof bits.unsigned_range k ltac:(blia).
+      eapply in_map_iff; exists (Z.to_nat (Zmod.unsigned k));
         rewrite ?in_seq; repeat split; rewrite ?Znat.Z2Nat.id;
-        try blia; try solve [eapply word.of_Z_unsigned].
+        try blia; try solve [eapply Zmod.of_Z_unsigned].
       apply nth_error_Some. congruence.
     Qed.
     Lemma get_of_list_word_at a xs i : get (of_list_word_at a xs) i
-      = nth_error xs (Z.to_nat (word.unsigned (word.sub i a))).
+      = nth_error xs (Z.to_nat (Zmod.unsigned (Zmod.sub i a))).
     Proof.
       cbv [of_list_word_at].
-      replace i with (word.add a (word.sub i a)) by ring.
+      replace i with (Zmod.add a (Zmod.sub i a)) by ring.
       rewrite get_map_keys_always_invertible, get_of_list_word.
       2: { intros ? ? H.
-           assert (A:word.sub (word.add a k) a = word.sub (word.add a k') a).
+           assert (A:Zmod.sub (Zmod.add a k) a = Zmod.sub (Zmod.add a k') a).
            { rewrite H; trivial. }
            ring_simplify in A; exact A. }
       f_equal. f_equal. f_equal. ring.
@@ -48,22 +52,22 @@ Module map.
     Lemma get_of_list_word_at_domain a xs i :
       get (of_list_word_at a xs) i <> None
       <->
-      (0 <= word.unsigned (word.sub i a) < Z.of_nat (length xs))%Z.
+      (0 <= Zmod.unsigned (Zmod.sub i a) < Z.of_nat (length xs))%Z.
     Proof.
-      pose proof word.unsigned_range (word.sub i a).
+      pose proof bits.unsigned_range (Zmod.sub i a) ltac:(blia).
       rewrite get_of_list_word_at, nth_error_Some.
       rewrite Nat2Z.inj_lt, ?Znat.Z2Nat.id; intuition.
     Qed.
 
     Lemma of_list_word_at_app a xs ys :
       of_list_word_at a (xs ++ ys) =
-      putmany (of_list_word_at (word.add a (word.of_Z (Z.of_nat (length xs)))) ys) (of_list_word_at a xs).
+      putmany (of_list_word_at (Zmod.add a (bits.of_Z width (Z.of_nat (length xs)))) ys) (of_list_word_at a xs).
     Proof.
       eapply map_ext; intros k.
       rewrite get_of_list_word_at.
-      pose proof word.unsigned_range (word.sub k a) as Hrange.
-      pose proof proj1 (nth_error_Some xs (Z.to_nat (word.unsigned (word.sub k a)))) as Hlength.
-      destruct (nth_error xs (Z.to_nat (word.unsigned (word.sub k a)))) as [v|] eqn:Hv.
+      pose proof bits.unsigned_range (Zmod.sub k a) ltac:(blia) as Hrange.
+      pose proof proj1 (nth_error_Some xs (Z.to_nat (Zmod.unsigned (Zmod.sub k a)))) as Hlength.
+      destruct (nth_error xs (Z.to_nat (Zmod.unsigned (Zmod.sub k a)))) as [v|] eqn:Hv.
       { specialize (Hlength ltac:(discriminate)).
         erewrite Properties.map.get_putmany_right;
           rewrite ?nth_error_app1, ?get_of_list_word_at by blia; eassumption. }
@@ -71,26 +75,26 @@ Module map.
       rewrite Properties.map.get_putmany_left; rewrite get_of_list_word_at; trivial.
       rewrite nth_error_app2 by assumption.
       f_equal.
-      transitivity (Z.to_nat (word.unsigned (word.sub k a) - Z.of_nat (length xs))); try blia.
+      transitivity (Z.to_nat (Zmod.unsigned (Zmod.sub k a) - Z.of_nat (length xs))); try blia.
       f_equal.
-      transitivity (word.unsigned (word.sub (word.sub k a) (word.of_Z (Z.of_nat (length xs))))).
+      transitivity (Zmod.unsigned (Zmod.sub (Zmod.sub k a) (bits.of_Z width (Z.of_nat (length xs))))).
       2: f_equal; ring.
       symmetry.
-      rewrite word.unsigned_sub.
-      rewrite (word.unsigned_of_Z (Z.of_nat (length xs))).
-      cbv [word.wrap]; rewrite (Z.mod_small (Z.of_nat (length xs))) by blia.
+      rewrite Zmod.unsigned_sub.
+      rewrite (Zmod.unsigned_of_Z (Z.of_nat (length xs))).
+      rewrite (Z.mod_small (Z.of_nat (length xs))) by blia.
       eapply Z.mod_small.
       split; blia.
     Qed.
 
     Lemma adjacent_arrays_disjoint a xs ys (H : (Z.of_nat (length xs) + Z.of_nat (length ys) <= 2^width)%Z) :
-      disjoint (of_list_word_at (word.add a (word.of_Z (Z.of_nat (length xs)))) ys) (of_list_word_at a xs).
+      disjoint (of_list_word_at (Zmod.add a (bits.of_Z width (Z.of_nat (length xs)))) ys) (of_list_word_at a xs).
     Proof.
       intros k y x Hy Hx.
       assert ((Z.of_nat (length xs) <= 2^width)%Z) by blia.
       assert ((Z.of_nat (length ys) <= 2^width)%Z) by blia.
-      pose proof word.unsigned_range (word.sub k a) as Hrange.
-      pose proof word.unsigned_range (word.sub k (word.add a (word.of_Z (Z.of_nat (length xs))))) as Hr2.
+      pose proof bits.unsigned_range (Zmod.sub k a) ltac:(blia) as Hrange.
+      pose proof bits.unsigned_range (Zmod.sub k (Zmod.add a (bits.of_Z width (Z.of_nat (length xs))))) ltac:(blia) as Hr2.
       rewrite get_of_list_word_at in *.
       repeat match goal with H: nth_error ?l ?i = Some _ |- _ =>
           let HH := fresh H in pose proof proj1 (nth_error_Some l i) as HH;
@@ -100,10 +104,10 @@ Module map.
       replace (length xs) with (Z.to_nat (Z.of_nat (length xs))) in Hx0 by blia; eapply Z2Nat.inj_lt in Hx0; try blia.
       replace (length ys) with (Z.to_nat (Z.of_nat (length ys))) in Hy0 by blia; eapply Z2Nat.inj_lt in Hy0; try blia.
 
-      replace (word.sub k (word.add a (word.of_Z (Z.of_nat (length xs)))))
-         with (word.sub (word.sub k a) (word.of_Z (Z.of_nat (length xs)))) in Hy0 by ring.
-      set (word.sub k a) as i in *.
-      rewrite (word.unsigned_sub i), word.unsigned_of_Z in Hy0; cbv [word.wrap] in Hy0.
+      replace (Zmod.sub k (Zmod.add a (bits.of_Z width (Z.of_nat (length xs)))))
+         with (Zmod.sub (Zmod.sub k a) (bits.of_Z width (Z.of_nat (length xs)))) in Hy0 by ring.
+      set (Zmod.sub k a) as i in *.
+      rewrite (Zmod.unsigned_sub i), Zmod.unsigned_of_Z in Hy0.
       rewrite Zminus_mod_idemp_r in Hy0.
       rewrite <-(Z_mod_plus _ 1), Z.mul_1_l in Hy0 by blia.
       rewrite Z.mod_small in Hy0; blia.
@@ -113,14 +117,14 @@ Module map.
       (a : word) (xs ys : list value)
       lxs (Hlxs : Z.of_nat (length xs) = lxs)
       : of_list_word_at a (xs ++ ys)
-      = putmany (of_list_word_at (word.add a (word.of_Z lxs)) ys) (of_list_word_at a xs).
+      = putmany (of_list_word_at (Zmod.add a (bits.of_Z width lxs)) ys) (of_list_word_at a xs).
     Proof. subst lxs; eapply of_list_word_at_app. Qed.
 
     Lemma adjacent_arrays_disjoint_n
       (a : word) (xs ys : list value)
       lxs (Hlxs : Z.of_nat (length xs) = lxs)
       (H : (Z.of_nat (length xs) + Z.of_nat (length ys) <= 2 ^ width)%Z)
-      : disjoint (of_list_word_at (word.add a (word.of_Z lxs)) ys) (of_list_word_at a xs).
+      : disjoint (of_list_word_at (Zmod.add a (bits.of_Z width lxs)) ys) (of_list_word_at a xs).
     Proof. subst lxs. auto using adjacent_arrays_disjoint. Qed.
 
     Lemma of_list_word_nil k : of_list_word_at k nil = empty.
@@ -129,19 +133,19 @@ Module map.
     Lemma of_list_word_singleton k v : of_list_word_at k (cons v nil) = put empty k v.
     Proof.
       cbv [of_list_word_at of_list_word seq length List.map of_func update].
-      rewrite word.unsigned_of_Z_0, Znat.Z2Nat.inj_0; cbv [MapKeys.map.map_keys nth_error].
+      rewrite Zmod.unsigned_0, Znat.Z2Nat.inj_0; cbv [MapKeys.map.map_keys nth_error].
       rewrite Properties.map.fold_singleton.
       f_equal; cbn [Z.of_nat].
-      eapply word.unsigned_inj; rewrite word.unsigned_add; cbv [word.wrap]; rewrite word.unsigned_of_Z_0, Z.add_0_r, Z.mod_small; trivial; eapply word.unsigned_range.
+      apply Zmod.unsigned_inj; rewrite Zmod.unsigned_add, Zmod.unsigned_0, Z.add_0_r, Z.mod_small; trivial; eapply bits.unsigned_range; blia.
     Qed.
 
     Import ListNotations.
     Local Notation "xs $@ a" := (of_list_word_at a xs) (at level 10, format "xs $@ a").
     Local Open Scope Z_scope.
     Local Coercion Z.of_nat : nat >-> Z.
-    Local Coercion word.unsigned : word.rep >-> Z.
+    Local Coercion Zmod.unsigned : Zmod >-> Z.
     Lemma of_list_word_at_cons b bs a :
-      (b :: bs)$@a = map.put (bs$@(word.add a (word.of_Z 1))) a b :> map.
+      (b :: bs)$@a = map.put (bs$@(Zmod.add a (bits.of_Z width 1))) a b :> map.
     Proof.
       change (b::bs) with ([b]++bs).
       rewrite of_list_word_at_app, of_list_word_singleton; cbn.
@@ -150,47 +154,47 @@ Module map.
 
     Lemma of_list_word_at_snoc b bs a
       (H : length bs < 2 ^ width)
-      : (bs ++ [b])$@a = map.put (bs$@a) (word.add a (word.of_Z (length bs))) b :> map.
+      : (bs ++ [b])$@a = map.put (bs$@a) (Zmod.add a (bits.of_Z width (length bs))) b :> map.
     Proof.
       rewrite of_list_word_at_app, of_list_word_singleton; cbn.
       rewrite map.putmany_comm; cycle 1.
       { intros k ? ?; rewrite map.get_put_dec.
-        destruct (@word.eqb _ _ _ _) eqn:Hbr;
+        destruct (@Zmod.eqb _ _ _) eqn:Hbr;
           autoforward with typeclass_instances in Hbr;
           rewrite ?map.get_empty, get_of_list_word_at; inversion 1; subst.
         intro HX.
         rewrite word.word_sub_add_l_same_l in HX.
         eapply List.nth_error_Some_bound_index in HX.
-        rewrite word.unsigned_of_Z in HX; cbv [word.wrap] in HX.
+        rewrite Zmod.unsigned_of_Z in HX.
         rewrite Z.mod_small in HX by Lia.lia; Lia.lia. }
       rewrite <-map.put_putmany_commute, map.putmany_empty_r. trivial.
     Qed.
 
     Lemma remove_head_of_list_word_at_cons b bs a
       (H : length bs < 2^width) :
-      map.remove ((b :: bs)$@a) a = bs$@(word.add a (word.of_Z 1)) :> map.
+      map.remove ((b :: bs)$@a) a = bs$@(Zmod.add a (bits.of_Z width 1)) :> map.
     Proof.
       rewrite of_list_word_at_cons, map.remove_put_same, map.remove_not_in; trivial.
       rewrite get_of_list_word_at. eapply List.nth_error_None.
-      enough (word.unsigned (word.sub a (word.add a (word.of_Z 1))) =2^width-1) by Lia.lia.
-      rewrite word.unsigned_sub, word.unsigned_add, word.unsigned_of_Z_1; cbv [word.wrap].
+      enough (Zmod.unsigned (Zmod.sub a (Zmod.add a (bits.of_Z width 1))) =2^width-1) by Lia.lia.
+      rewrite Zmod.unsigned_sub, Zmod.unsigned_add, bits.unsigned_1 by Lia.lia.
       rewrite Zdiv.Zminus_mod_idemp_r.
       replace (a - (a + 1)) with (Z.opp 1) by Lia.lia.
       rewrite Zdiv.Z_mod_nz_opp_full; rewrite ?Z.mod_small; ssplit; trivial; try Lia.lia.
-      all : enough (2^1 <= 2^width) by Lia.lia; pose proof word.width_pos.
+      all : enough (2^1 <= 2^width) by Lia.lia.
       all : eapply Z.pow_le_mono_r; Lia.lia.
     Qed.
 
     Lemma remove_last_of_list_word_at_snoc b bs a
       (H : length bs < 2 ^ width)
-      a' (Ha' : a' = word.add a (word.of_Z (length bs)))
+      a' (Ha' : a' = Zmod.add a (bits.of_Z width (length bs)))
       : map.remove ((bs ++ [b])$@a) a' = bs$@a :> map.
     Proof.
       subst a'.
       rewrite of_list_word_at_snoc, map.remove_put_same, map.remove_not_in; trivial.
       rewrite get_of_list_word_at; eapply List.nth_error_None.
       rewrite word.word_sub_add_l_same_l.
-      rewrite word.unsigned_of_Z; cbv [word.wrap]; rewrite Z.mod_small; Lia.lia.
+      rewrite Zmod.unsigned_of_Z; rewrite Z.mod_small; Lia.lia.
     Qed.
   End __.
 End map.
